

Ashish Upadhyay

CST SPL 1

Roll no. 16

DAA Tutorial 1

Ans. ① Asymptotic notations are the mathematical notations used to describe the running time of an algorithm when the input tends towards a particular limiting value.

Asymptotic notations are of 3 types:

① Big O notation: It is the upper bound of the running time of an algorithm and it gives the worst ^{case} complexity.

② Omega Notation: It is the lower bound of the running time of an algorithm and gives the best case complexity of an algorithm.

③ Θ - Notation (Theta): This encloses the function from above and below. It is used to determine average case complexity of an algorithm.

e.g. The

Ans. ② $i = 1, 2, 4, 8, 16, \dots, n$

This is a G.P.

$$a_k = ar^{k-1}$$

$$a=1, r=2$$

$$n = 2^{k-1}$$

$$\Rightarrow k = \log_2 n + 1$$

$$\therefore T(n) = O(\log_2 n)$$

Ans.

Ans. (3)

$$T(n) = 3T(n-1) \text{ --- (1)}$$

$$T(0) = 1 \text{ --- (2)}$$

putting $n = n-1$ in (1)

$$T(n-1) = 3T(n-2) \text{ --- (3)}$$

putting (3) in (1)

$$T(n) = 3(3T(n-2)) = 3^2 T(n-2) \text{ --- (4)}$$

putting ~~n~~ $n = n-2$ in equ. (1)

$$T(n-2) = 3T(n-2-1) = 3T(n-3) \text{ --- (5)}$$

putting value of $T(n-2)$ from (5) to (4)

$$T(n) = 3^2 [3T(n-3)] = 3^3 T(n-3)$$

\therefore we can see the below trend:

$$T(n) = \cancel{3^k} 3^k T(n-k)$$

$$\text{Let } n-k=0 \therefore n=k$$

$$T(n) = 3^n T(0)$$

$$\text{as } T(0) = 1$$

$$\therefore T(n) = 3^n$$

$$T(n) = O(3^n)$$

Ans.

Ans (4.) $T(n) = [2T(n-1) - 1 ; \because n > 0 ; \text{otherwise } 1]$

$$T(n) = 2T(n-1) - 1 \quad \text{--- (1)}$$

$$T(0) = 1 \quad \text{--- (2)}$$

putting $n = n-1$ in (1):

$$T(n-1) = 2T(n-2) - 1 \quad \text{--- (3)}$$

putting values in (3) to (1)

$$T(n) = 2(2(T(n-2) - 1) - 1)$$

$$T(n) = 2^2 T(n-2) - 2 - 1 \quad \text{--- (4)}$$

putting value $n = n-2$ in (1):

$$T(n-2) = 2T(n-2-1) - 1$$

$$= 2(T(n-3)) - 1 \quad \text{--- (5)}$$

putting value of (5) in (4):

$$T(n) = 2^2 [2T(n-3) - 1] - 2 - 1$$

$$T(n) = 2^3 T(n-1) - 2^2 - 2^1 - 2^0 \quad \text{--- (6)}$$

\therefore the trend is as below:

$$T(n) = 2^k T(n-k) - 2^{k-1} - 2^{k-2} - 2^{k-3} - \dots - 2^0$$

$$\text{let } n-k=0$$

$$\therefore n=k$$

$$T(n) = 2^n T(n-n) - 2^{n-1} - 2^{n-2} - \dots - 2^0$$

~~as~~

$$T(n) = 2^n T(0) - 2^{n-1} - 2^{n-2} - \dots - 2^0$$

$$\Rightarrow T(n) = 2^n - 2^{n-1} - 2^{n-2} - \dots - 2^0 \quad \{T(0) = 1\}$$

$$\cancel{T(n) = 2^n - 2^{n-1} T(n)} = 2^n - (1 + 2^1 + 2^2 + \dots + 2^{n-1})$$

$$T(n) = 2^n - \left(\frac{1 \times (2^n - 1)}{2 - 1} \right)$$

$$T(n) = 2^n - 2^n + 1$$

$$\therefore T(n) = \underline{\underline{O(1)}} \quad \underline{\underline{Ans.}}$$

Ans. (5)

$$\text{for } i=1, s=1$$

$$\text{for } i=2, s=1+2 \quad s=3$$

$$\text{for } i=3, s=1+2+3 \quad s=6$$

\therefore this is the sum of 'n' natural nos.

$$s = \cancel{1+2+\dots+n} \quad \frac{k(k+1)}{2}$$

To stop the iteration, s should be greater than n.
 \therefore

$$\frac{k(k+1)}{2} > n$$

$$\Rightarrow k^2 + k > 2n$$

$$\Rightarrow k^2 > n$$

$$\Rightarrow k > \sqrt{n}$$

$$\therefore \underline{\underline{O(k) = \sqrt{n}}} \quad \underline{\underline{Ans.}}$$

Ans. (6)

$$i = 1, 2, 3, \dots, n$$

$$i^2 = 1, 4, 9, \dots, n^2$$

$$\therefore i^2 \leq n \quad \text{or } i \leq \sqrt{n}$$

$$\text{now, } a_k = a + (k-1)d$$

$$\rightarrow a=1, d=1$$

$$a_k \leq \sqrt{n}$$

$$\sqrt{n} = 1 + (k-1) \cdot 1$$

$$\sqrt{n} = k$$

$$\therefore T(n) = \underline{\underline{O(\sqrt{n})}} \quad \underline{\underline{Ans.}}$$

Ans. 7

(i)

(j)

(k)

$$\frac{n}{2}$$

$$(\log_2 n)$$

$$(\log_2 n)$$

:

:

:

n

$$\left(\frac{n}{2} + 1\right) \text{ times}$$

$$\log_2 n$$

$$(\log_2 n)$$

$$O(i * j * k) = O\left(\left(\frac{n}{2} + 1\right) \times \log_2 n \times \log_2 n\right)$$

$$= O\left(\left(\frac{n}{2} + 1\right) \times (\log_2 n)^2\right)$$

$$\therefore T(n) = O\left(n (\log_2 n)^2\right) \quad \underline{\underline{\text{Ans.}}}$$

Ans. 8

$$T(n) = T(n-3) + n^2 \quad \text{--- (1)}$$

$$T(1) = 1 \quad \text{--- (2)}$$

Putting $n=n-3$ in (1):

$$T(n-3) = T(n-3-3) + (n-3)^2 \quad \text{--- (3)}$$

Putting (3) in (1):

$$T(n) = T(n-6) + (n-3)^2 + n^2 \quad \text{--- (4)}$$

Putting $n=n-6$ in (1):

$$T(n-6) = T(n-6-6) + (n-6)^2 \quad \text{--- (5)}$$

Putting (5) in (4):

$$T(n) = T(n-12) + (n-6)^2 + (n-3)^2 + n^2$$

after generalization we get:

$$T(n) = T(n-3k) + (n-3(k-1))^2 + (n-3(k-2))^2 + \dots + n^2$$

$$\text{Let } n-3k=1,$$

$$\frac{n-1}{3} = k$$

$$T(n) = T(1) + \left(n-3\left(\frac{n-1}{3}-1\right)\right)^2 + \left(n-3\left(\frac{n-1}{3}-2\right)\right)^2 + \dots + n^2$$

$$T(n) = T(1) + [n - \cancel{(n-1)} - 3]^2 + [n - (\cancel{n-1} - 6)]^2 + [n - (n-1-1)]^2 + \dots + n^2$$

$$T(n) = 1 + (3+1)^2 + (6+1)^2 + \dots + n^2$$

$$T(n) = 1 + 4^2 + 6^2 + \dots + n^2$$

$$= n^2 + \dots$$

$$\therefore T(n) = O(n^2)$$

Ans.